src/Prototype/LanguageFacts.v
@@ -1,29 +1,249 @@
 Require Import Bool List String Peano_dec.
 Require Import FunctionalExtensionality.
-Require Import Tactics FMap Language.
+Require Import FMap Tactics Language.
 
-Section Facts.
+Set Implicit Arguments.
+
+Lemma forall_filter:
+  forall {A} (l: list A) P (f: A -> bool),
+    Forall P l -> Forall P (filter f l).
+Proof.
+  induction l; simpl; intros; auto.
+  inv H; destruct (f a); auto.
+Qed.
+
+Lemma forall_app:
+  forall {A} (l1 l2: list A) P,
+    Forall P l1 -> Forall P l2 -> Forall P (l1 ++ l2).
+Proof.
+  induction l1; simpl; intros; auto.
+  inv H; constructor; auto.
+Qed.
+
+Section Label.
   Variable MsgT: Type.
   Hypothesis (msgT_dec: forall m1 m2: MsgT, {m1 = m2} + {m1 <> m2}).
   Variable ValT: Type.
   Hypothesis (valT_dec: forall m1 m2: ValT, {m1 = m2} + {m1 <> m2}).
   Variable StateT: Type.
 
-  Local Notation Msg := (Msg MsgT ValT).
-  Local Notation Label := (Label MsgT ValT).
-  Local Notation step_sys := (step_sys msgT_dec valT_dec).
+  Local Notation Object := (Object MsgT ValT StateT).
   Local Notation System := (System MsgT ValT StateT).
 
-  Definition ValidLabel (l: Label) :=
-    match lbl_hdl l with
-    | Some hdl => lbl_ins l = nil /\ ValidOuts (msgTo (msg_id hdl)) (lbl_outs l)
-    | None => lbl_outs l = nil
-    end.
+  Local Notation Label := (Label MsgT ValT).
+  Local Notation emptyLabel := (emptyLabel MsgT ValT).
+  Local Notation combineLabel := (combineLabel msgT_dec valT_dec).
+
+  Local Notation step_sys := (step_sys msgT_dec valT_dec).
+
+  Lemma step_obj_validLabel:
+    forall (obj: Object) st1 mf1 lbl st2 mf2,
+      step_obj obj st1 mf1 lbl st2 mf2 -> ValidLabel lbl.
+  Proof.
+    intros; inv H; cbn; auto.
+  Qed.
+
+  Lemma combineLabel_validLabel:
+    forall lbl1 lbl2,
+      ValidLabel lbl1 -> ValidLabel lbl2 ->
+      ValidLabel (combineLabel lbl1 lbl2).
+  Proof.
+    unfold ValidLabel, combineLabel;
+      destruct lbl1 as [ins1 hdl1 outs1], lbl2 as [ins2 hdl2 outs2]; simpl; intros.
+    destruct hdl1, hdl2; subst; simpl; reflexivity.
+  Qed.
 
   Lemma step_sys_validLabel:
-    forall (sys: System) st1 l st2, step_sys sys st1 l st2 -> ValidLabel l.
+    forall (sys: System) st1 lbl st2,
+      step_sys sys st1 lbl st2 -> ValidLabel lbl.
   Proof.
-  Admitted.
+    induction 1; simpl; intros.
+    - eapply step_obj_validLabel; eauto.
+    - apply combineLabel_validLabel; auto.
+  Qed.
+  
+  Lemma combineLabel_emptyLabel_1:
+    forall l, ValidLabel l -> combineLabel emptyLabel l = l.
+  Proof.
+    unfold ValidLabel; destruct l as [ins hdl outs]; cbn; intros.
+    destruct hdl; subst; auto.
+    f_equal.
+    induction outs; simpl; auto.
+    f_equal; auto.
+  Qed.
+  
+  Lemma combineLabel_emptyLabel_2:
+    forall l, ValidLabel l -> combineLabel l emptyLabel = l.
+  Proof.
+    unfold ValidLabel, combineLabel; destruct l as [ins hdl outs]; cbn; intros.
+    destruct hdl; subst; auto.
+    - f_equal.
+      induction outs; simpl; auto.
+      f_equal; auto.
+    - rewrite app_nil_r; reflexivity.
+  Qed.
 
-End Facts.
+End Label.
+  
+Section Singleton.
+  Variable MsgT: Type.
+  Hypothesis (msgT_dec: forall m1 m2: MsgT, {m1 = m2} + {m1 <> m2}).
+  Variable ValT: Type.
+  Hypothesis (valT_dec: forall m1 m2: ValT, {m1 = m2} + {m1 <> m2}).
+  Variable StateT: Type.
+
+  Local Notation Object := (Object MsgT ValT StateT).
+  Local Notation System := (System MsgT ValT StateT).
+
+  Local Notation emptyLabel := (emptyLabel MsgT ValT).
+  Local Notation step_sys := (step_sys msgT_dec valT_dec).
+
+  Lemma step_obj_msgTo:
+    forall (obj: Object) st1 mf1 lbl st2 mf2,
+      step_obj obj st1 mf1 lbl st2 mf2 ->
+      Forall (fun m => msgTo (msg_id m) = obj_idx obj) (lbl_ins lbl) /\
+      Forall (fun m => msgTo (msg_id m) <> obj_idx obj) (lbl_outs lbl).
+  Proof.
+    intros; inv H.
+    - cbn; split; constructor.
+    - cbn; split; [constructor|].
+      destruct H6.
+      eapply Forall_impl; try eassumption.
+      simpl; intros; destruct H7; auto.
+    - cbn; split; constructor; auto.
+  Qed.
+
+  Lemma step_sys_singleton_msgTo:
+    forall (obj: Object) s1 lbl s2,
+      step_sys [obj] s1 lbl s2 ->
+      Forall (fun m => msgTo (msg_id m) = obj_idx obj) (lbl_ins lbl) /\
+      Forall (fun m => msgTo (msg_id m) <> obj_idx obj) (lbl_outs lbl).
+  Proof.
+    induction 1.
+    - dest_in; eapply step_obj_msgTo; eauto.
+    - destruct lbl1 as [ins1 hdl1 outs1], lbl2 as [ins2 hdl2 outs2].
+      unfold combineLabel; simpl in *.
+      destruct hdl1, hdl2; simpl.
+      + split; constructor.
+      + split; [constructor|].
+        dest; apply forall_filter; auto.
+      + split; [constructor|].
+        dest; apply forall_filter; auto.
+      + split; [|constructor].
+        dest; apply forall_app; auto.
+  Qed.
+
+  Lemma step_obj_singleton_no_combs:
+    forall (obj: Object) st11 mf11 lbl1 st12 mf12 st21 mf21 lbl2 st22 mf22,
+      step_obj obj st11 mf11 lbl1 st12 mf12 ->
+      step_obj obj st21 mf21 lbl2 st22 mf22 ->
+      (lbl1 = emptyLabel \/ lbl2 = emptyLabel \/ ~ CombinableLabel lbl1 lbl2).
+  Proof.
+    intros.
+    inv H; [tauto| |].
+    - inv H0; [tauto|tauto|].
+      right; right.
+      cbn; intro Hx.
+      specialize (Hx emsg (or_introl eq_refl)).
+      destruct H7.
+      eapply Forall_forall in H0; eauto.
+      destruct H0.
+      rewrite H in H8; elim H8; reflexivity.
+    - inv H0; [tauto| |].
+      + right; right.
+        cbn; intro Hx.
+        specialize (Hx emsg (or_introl eq_refl)).
+        destruct H7.
+        eapply Forall_forall in H0; eauto.
+        destruct H0.
+        rewrite H1 in H8; elim H8; reflexivity.
+      + right; right.
+        cbn; intro Hx.
+        rewrite H, H1 in Hx.
+        inv Hx; elim H3.
+        left; reflexivity.
+  Qed.
+
+  Lemma step_sys_singleton_no_combs:
+    forall (obj: Object) st11 lbl1 st12 st21 lbl2 st22,
+      step_sys [obj] st11 lbl1 st12 ->
+      step_sys [obj] st21 lbl2 st22 ->
+      (lbl1 = emptyLabel \/ lbl2 = emptyLabel \/ ~ CombinableLabel lbl1 lbl2).
+  Proof.
+    intros.
+    pose proof (step_sys_validLabel H).
+    pose proof (step_sys_validLabel H0).
+    pose proof (step_sys_singleton_msgTo H).
+    pose proof (step_sys_singleton_msgTo H0).
+    dest.
+
+    unfold ValidLabel in *;
+      destruct lbl1 as [ins1 hdl1 outs1], lbl2 as [ins2 hdl2 outs2]; simpl in *.
+
+    destruct hdl1; subst.
+    - destruct hdl2; subst; auto.
+      destruct ins2; auto.
+      right; right; cbn.
+      intro Hx; apply SubList_cons_inv in Hx; dest.
+      eapply Forall_forall in H6; eauto.
+      inv H4; rewrite H9 in H6; auto.
+    - destruct ins1; auto.
+      destruct hdl2; subst.
+      + right; right; cbn.
+        intro Hx; apply SubList_cons_inv in Hx; dest.
+        eapply Forall_forall in H5; eauto.
+        inv H3; rewrite H9 in H5; auto.
+      + destruct ins2; auto.
+        right; right; cbn.
+        inv H3; inv H4.
+        intro Hx; inv Hx; elim H4.
+        rewrite map_app; simpl; apply in_or_app.
+        right; left.
+        rewrite H3, H7; reflexivity.
+  Qed.
+      
+  Lemma step_obj_singleton_step_sys:
+    forall (obj: Object) st1 mf1 lbl st2 mf2,
+      step_obj obj st1 mf1 lbl st2 mf2 ->
+      step_sys [obj] {| st_oss := [obj_idx obj <- st1];
+                        st_msgs := [obj_idx obj <- mf1] |}
+               lbl {| st_oss := [obj_idx obj <- st2];
+                      st_msgs := [obj_idx obj <- mf2] |}.
+  Proof.
+    intros.
+    replace [obj_idx obj <- st2] with [obj_idx obj <- st1]+[obj_idx obj <- st2] by meq.
+    replace [obj_idx obj <- mf2] with [obj_idx obj <- mf1]+[obj_idx obj <- mf2] by meq.
+    eapply SsLift; eauto.
+    - left; reflexivity.
+    - mred.
+    - mred.
+  Qed.
+      
+  Lemma step_sys_singleton_step_obj:
+    forall (obj: Object) s1 lbl s2,
+      step_sys [obj] s1 lbl s2 ->
+      exists st1 mf1 st2 mf2,
+        (st_oss s1)@[obj_idx obj] = Some st1 /\
+        (st_msgs s1)@[obj_idx obj] = Some mf1 /\
+        (st_oss s2)@[obj_idx obj] = Some st2 /\
+        (st_msgs s2)@[obj_idx obj] = Some mf2 /\
+        step_obj obj st1 mf1 lbl st2 mf2.
+  Proof.
+    induction 1; simpl; intros; subst.
+    - dest_in.
+      do 4 eexists; repeat split; eauto; mred.
+    - pose proof (step_sys_singleton_no_combs H H0).
+      destruct H4 as [|[|]]; subst.
+      + unfold DisjointState in H1, H2; dest.
+        do 4 eexists; repeat split; try (apply M.Disj_find_union_2; eauto; fail).
+        rewrite combineLabel_emptyLabel_1; auto.
+        eapply step_obj_validLabel; eauto.
+      + unfold DisjointState in H1, H2; dest.
+        do 4 eexists; repeat split; try (apply M.Disj_find_union_1; eauto; fail).
+        rewrite combineLabel_emptyLabel_2; auto.
+        eapply step_obj_validLabel; eauto.
+      + elim H4; auto.
+  Qed.
+
+End Singleton.
 
